Hoare/HoareTripleForInstructions3.thy
@@ -1,0 +1,76 @@
+(*
+   Copyright 2017 Myriam Begel
+
+   Licensed under the Apache License, Version 2.0 (the "License");
+   you may not use this file except in compliance with the License.
+   You may obtain a copy of the License at
+
+       http://www.apache.org/licenses/LICENSE-2.0
+
+   Unless required by applicable law or agreed to in writing, software
+   distributed under the License is distributed on an "AS IS" BASIS,
+   WITHOUT WARRANTIES OR CONDITIONS OF ANY KIND, either express or implied.
+   See the License for the specific language governing permissions and
+   limitations under the License.
+*)
+
+theory "HoareTripleForInstructions3"
+
+imports "HoareTripleForInstructions"
+"../attic/BasicBlocks"
+"../EvmFacts"
+
+begin
+type_synonym pred = "(state_element set \<Rightarrow> bool)"
+
+(* We define here the program logic for BLOCKSs *)
+(* We start with Hoare triples valid for the execution of one instruction *)
+
+(* We have to add more instructions here *)
+inductive triple_inst_pc :: "pred \<Rightarrow> pos_inst \<Rightarrow> pred \<Rightarrow> bool" where
+  inst_jumpdest :
+    "triple_inst_pc
+      (\<langle> h \<le> 1024 \<and> Gjumpdest \<le> g \<and> m \<ge> 0\<rangle> \<and>*
+       continuing \<and>* memory_usage m \<and>* program_counter n \<and>*
+       stack_height h \<and>* gas_pred g \<and>* rest)
+      (n, Pc JUMPDEST)
+      (continuing \<and>* program_counter (n + 1) \<and>*
+       memory_usage m \<and>* stack_height h \<and>*
+       gas_pred (g - Gjumpdest) \<and>* rest)"
+
+inductive triple_inst_stack :: "pred \<Rightarrow> pos_inst \<Rightarrow> pred \<Rightarrow> bool" where
+  inst_push_n :
+    "triple_inst_stack
+      (\<langle> h \<le> 1023 \<and> length lst > 0 \<and> 32 \<ge> length lst \<and> Gverylow \<le> g \<and> m \<ge> 0\<rangle> \<and>*
+       continuing \<and>* program_counter n \<and>*
+       memory_usage m \<and>* stack_height h \<and>*
+       gas_pred g \<and>* rest)
+      (n, Stack (PUSH_N lst))
+      (continuing \<and>* memory_usage m \<and>*
+       program_counter (n + 1 + int (length lst)) \<and>*
+       stack_height (Suc h) \<and>* gas_pred (g - Gverylow) \<and>*
+       stack h (word_rcat lst) \<and>* rest)"
+
+inductive triple_inst_misc :: "pred \<Rightarrow> pos_inst \<Rightarrow> pred \<Rightarrow> bool" where
+ inst_stop :
+    "triple_inst_misc
+      (\<langle> h \<le> 1024 \<and> 0 \<le> g \<and> m \<ge> 0\<rangle> \<and>* continuing \<and>* memory_usage m \<and>*
+       program_counter n \<and>* stack_height h \<and>* gas_pred g \<and>* rest)
+      (n, Misc STOP)
+      (stack_height h \<and>* not_continuing \<and>* memory_usage m \<and>*
+       program_counter n \<and>* action (ContractReturn []) \<and>*
+       gas_pred g \<and>* rest)"
+
+
+inductive triple_inst :: "pred \<Rightarrow> pos_inst \<Rightarrow> pred \<Rightarrow> bool" where
+  inst_misc :
+    "triple_inst_misc p (n, Misc i) q \<Longrightarrow> triple_inst p (n, Misc i) q"
+| inst_pc :
+    "triple_inst_pc p (n, Pc i) q \<Longrightarrow> triple_inst p (n, Pc i) q"
+| inst_stack :
+    "triple_inst_stack p (n, Stack i) q \<Longrightarrow> triple_inst p (n, Stack i) q"
+| inst_strengthen_pre:
+    "triple_inst p i q \<Longrightarrow> (\<And>s. r s \<longrightarrow> p s) \<Longrightarrow> triple_inst r i q"
+| inst_false_pre:
+    "triple_inst \<langle>False\<rangle> i post"
+end
